code/experimental/salsa-family/Chacha20.Vec128.fsti
@@ -2,11 +2,13 @@ module Chacha20.Vec128
 
 
 open FStar.Buffer
-
+open FStar.UInt32
 
 let uint8_p = buffer Hacl.UInt8.t
 
 #reset-options "--max_fuel 0 --z3rlimit 20"
+
+let op_String_Access h (b:uint8_p{live h b}) = Hacl.Spec.Endianness.reveal_sbytes (as_seq h b)
 
 val chacha20:
   output:uint8_p ->
@@ -18,10 +20,5 @@ val chacha20:
   Stack unit
     (requires (fun h -> live h output /\ live h plain /\ live h key /\ live h nonce))
     (ensures (fun h0 _ h1 -> live h1 output /\ live h0 plain /\ live h0 key /\ live h0 nonce
-      /\ modifies_1 output h0 h1 /\ (
-      let output = as_seq h1 output in
-      let key = as_seq h0 key in
-      let nonce = as_seq h0 nonce in
-      let ctr = UInt32.v ctr in      
-      let plain = as_seq h0 plain in
-      output == Spec.Chacha20.chacha20_encrypt_bytes key nonce ctr plain) ))
+      /\ modifies_1 output h0 h1 /\
+      h1.[output] == Spec.Chacha20.chacha20_encrypt_bytes h0.[key] h0.[nonce] (v ctr) h0.[plain] ))
